theories/rust_typing/ltypes.v
@@ -24,24 +24,26 @@ Section enum.
     (* out of the current refinement, extract the tag *)
     enum_tag : rt → var_name;
     (* out of the current refinement, extract the component type and refinement *)
-    enum_ty : rt → sigT (λ rt' : Type, type rt' * rt')%type;
+    enum_rt : rt → Type;
+    enum_ty : ∀ r, type (enum_rt r);
+    enum_r : ∀ r, enum_rt r;
     (* convenience function: given the variant name, also project out the type *)
     enum_tag_ty : var_name → option (sigT type);
     (* explicitly track the lifetimes each of the variants needs -- needed for sharing *)
     enum_lfts : list lft;
     enum_wf_E : elctx;
-    enum_lfts_complete : ∀ (r : rt), ty_lfts (projT2 (enum_ty r)).1 ⊆ enum_lfts;
-    enum_wf_E_complete : ∀ (r : rt), ty_wf_E (projT2 (enum_ty r)).1 ⊆ enum_wf_E;
+    enum_lfts_complete : ∀ (r : rt), ty_lfts (enum_ty r) ⊆ enum_lfts;
+    enum_wf_E_complete : ∀ (r : rt), ty_wf_E (enum_ty r) ⊆ enum_wf_E;
     enum_tag_compat : ∀ (r : rt) (variant : var_name),
       enum_tag r = variant →
-      ∃ rte lte re,
-        enum_ty r = existT rte (lte, re) ∧
-        enum_tag_ty variant = Some (existT rte lte)
+      enum_tag_ty variant = Some (existT (enum_rt r) (enum_ty r))
   }.
   Global Arguments mk_enum {_ _}.
   Global Arguments enum_rt_inhabited {_}.
   Global Arguments enum_els {_}.
   Global Arguments enum_tag {_}.
+  Global Arguments enum_rt {_}.
+  Global Arguments enum_r {_}.
   Global Arguments enum_ty {_}.
   Global Arguments enum_tag_ty {_}.
   Global Arguments enum_lfts {_}.
@@ -56,11 +58,11 @@ Section enum.
     projT2 (enum_tag_ty' en v).
 
   Definition enum_variant_rt {rt} (en : enum rt) (r : rt) : Type :=
-    projT1 (enum_ty en r).
+    (enum_rt en r).
   Definition enum_variant_rfn {rt} (en : enum rt) (r : rt) : (enum_variant_rt en r) :=
-    snd (projT2 (enum_ty en r)).
+    ((enum_r en r)).
   Definition enum_variant_type {rt} (en : enum rt) (r : rt) : type (enum_variant_rt en r) :=
-    fst (projT2 (enum_ty en r)).
+    ((enum_ty en r)).
 
   Definition enum_lookup_tag {rt} (e : enum rt) (r : rt) :=
     els_lookup_tag e.(enum_els) (e.(enum_tag) r).
@@ -76,25 +78,14 @@ Section enum.
     enum_tag_rt en tag = enum_variant_rt en r.
   Proof.
     intros ->.
-    edestruct (enum_tag_compat _ en r) as (rte & lte & re & Ha & Hb); first done.
     rewrite /enum_tag_rt /enum_variant_rt /enum_tag_ty'.
-    rewrite Ha Hb/=//.
+    rewrite (enum_tag_compat _ en r); done.
   Defined.
 
-  Lemma enum_tag_ty_Some {rt} (en : enum rt) r {rte : Type} (tye : type rte) (re : rte) :
-    enum_ty en r = (existT rte (tye, re)) →
-    enum_tag_ty en (enum_tag en r) = Some (existT rte tye).
+  Lemma enum_tag_ty_Some {rt} (en : enum rt) r :
+    enum_tag_ty en (enum_tag en r) = Some (existT (enum_rt en r) (enum_ty en r)).
   Proof.
-    destruct (enum_tag_compat _ en r _ eq_refl) as (rte' & lte' & re' & -> & ->).
-    intros Ha. injection Ha. intros _ _ ->.
-    apply existT_inj in Ha. injection Ha as -> ->.
-    done.
-  Qed.
-  Lemma enum_tag_ty_Some' {rt} (en : enum rt) r :
-    enum_tag_ty en (enum_tag en r) = Some (existT (projT1 (enum_ty en r)) (fst $ projT2 (enum_ty en r))).
-  Proof.
-    eapply (enum_tag_ty_Some _ _ _ (snd $ projT2 (enum_ty en r))).
-    destruct (enum_ty en r) as [? [??]]; done.
+    by rewrite (enum_tag_compat _ en r _ eq_refl).
   Qed.
 
   Import EqNotations.
@@ -102,11 +93,11 @@ Section enum.
     enum_tag_type en (enum_tag en r) = rew <-[type] (enum_tag_rt_variant_rt_eq en r _ eq_refl) in enum_variant_type en r.
   Proof.
     (*destruct (enum_ty en r) as [rte [lte re]] eqn:Heq.*)
-    destruct (enum_tag_compat _ en r (enum_tag en r)) as (rte & lte & re & Ha & Hb); first done.
     rewrite /enum_tag_type/enum_variant_type/enum_tag_ty'.
+    specialize (enum_tag_compat _ en r (enum_tag en r) eq_refl) as Hb.
     generalize (enum_tag_rt_variant_rt_eq en r (enum_tag en r) eq_refl) as Heq.
     rewrite /enum_tag_rt /enum_tag_ty' /enum_variant_rt.
-    rewrite Ha Hb. simpl.
+    rewrite Hb. simpl.
     intros Heq. rewrite (UIP_refl _ _ Heq); done.
   Qed.
 End enum.
